coqjit/assume_insertion_proof.v
@@ -1,0 +1,1017 @@
+(* Correctness of the Assume Insertion pass *)
+(* A pass of the middle-end optimizer *)
+(* Inserts an Assume insertion just after an Anchor *)
+
+Require Import internal_simulations.
+Require Import sem_properties.
+Require Import assume_insertion.
+Require Import Coq.MSets.MSetPositive.
+Require Import def_regs.
+Require Import common.
+Require Import IR.
+Require Import IRinterpreter.
+Require Import Errors.
+Require Import monad.
+Require Import monad_impl.
+Require Import mixed_sem.
+Require Import sem_properties.
+Require Import customSmallstep.
+
+Require Import IRtoRTLblock_proof.
+(* so we can resue the addstk typing of the monads *)
+(* TODO: We could get that in another file *)
+
+
+(** * Matching the stack and properties  *)
+(* Matching stackframes: a version may have been replaced with its optimized version *)
+Inductive match_stackframe (v:version) (fid:fun_id) (guard:expr) (ancl:label) (params:list reg): stackframe -> stackframe -> Prop :=
+| frame_same:
+    forall sf, (match_stackframe v fid guard ancl params) sf sf
+| frame_opt:
+    forall r lbl rm vins abs
+      (AS_INSERT: insert_assume_version v fid guard ancl params = OK vins)
+      (DEFREGS: defined_regs_analysis (ver_code v) params (ver_entry v) = Some abs)
+      (DEF: forall retval, defined (rm#r<-retval) (def_absstate_get lbl abs)),
+      (match_stackframe v fid guard ancl params) (IR_SF (r, v, lbl, rm)) (IR_SF (r, vins, lbl, rm)).
+
+(* Generalizing match_stackframe to the entire stack *)
+Inductive match_stack (v:version) (fid:fun_id) (guard:expr) (ancl:label) (params:list reg): stack -> stack -> Prop :=
+| match_nil:
+    (match_stack v fid guard ancl params) nil nil
+| match_cons:
+    forall s s' sf sf'
+      (MS: (match_stack v fid guard ancl params) s s')
+      (MSF: (match_stackframe v fid guard ancl params) sf sf'),
+      (match_stack v fid guard ancl params) (sf::s) (sf'::s').
+
+Lemma match_stack_same:
+  forall s v fid guard ancl params,
+    (match_stack v fid guard ancl params) s s.
+Proof.
+  intros s v fid guard ancl. induction s; constructor. auto. constructor.
+Qed.
+
+Lemma match_app:
+  forall synth s s' v fid guard ancl params,
+    (match_stack v fid guard ancl params) s s' ->
+    (match_stack v fid guard ancl params) (synth++s) (synth++s').
+Proof.
+  intros. induction synth.
+  - simpl. auto.
+  - repeat rewrite <- app_comm_cons. apply match_cons. auto. constructor.
+Qed.
+
+Lemma app_match:
+  forall synth synthopt s s' v fid guard ancl params,
+    (match_stack v fid guard ancl params) s s' ->
+    (match_stack v fid guard ancl params) synth synthopt ->
+    (match_stack v fid guard ancl params) (synth++s) (synthopt++s').
+Proof.
+  intros. induction H0.
+  - simpl. auto.
+  - repeat rewrite <- app_comm_cons. apply match_cons; auto.
+Qed.
+
+(** * Index and order used in the simulation *)
+(* There is one stuttering step for each inserted Anchor *)
+Inductive as_index: Type :=
+| One : as_index
+| Zero: as_index.
+
+Inductive as_order: as_index -> as_index -> Type :=
+| order: as_order Zero One.
+
+Lemma wfounded: well_founded as_order.
+Proof.
+  unfold well_founded. intros a. constructor. intros y H. inv H. constructor. intros y H. inv H.
+Qed.
+
+Lemma trans: Relation_Definitions.transitive _ as_order.
+Proof.
+  unfold Relation_Definitions.transitive. intros x y z H H0. inv H. inv H0.
+Qed.
+
+
+(** * The match_states relation  *)
+(* This proof is a backward internal simulation.
+   At the Anchor instruction, we take a stuttering step if the Assume succeeds
+   If it fails, we take a single step to the target version.
+
+<<
+                 
+       st1 --------------- st2
+        |                   |
+       t|(1 or 2 steps)     |t
+        |                   |
+        v                   v
+       st1'--------------- st2'
+                 
+>>
+*)
+
+Inductive match_states (p:program) (v:version) (fid:fun_id) (guard: expr) (ancl:label) (params:list reg): as_index -> mixed_state -> mixed_state -> Prop :=
+                                        
+| assume_match:                     (* matching at the assume instruction *)
+    forall vins stk stk' heap rm fresh fa la vm next (* newver *) newrm abs
+      (MATCHSTACK: (match_stack v fid guard ancl params) stk stk')
+      (OPT: insert_assume_version v fid guard ancl params = OK vins)
+      (DEFREGS: defined_regs_analysis (ver_code v) params (ver_entry v) = Some abs)
+      (DEF: defined rm (def_absstate_get ancl abs))
+      (VALIDATE: validator v ancl guard params = OK tt)
+      (FS_OPT: (ver_code vins) # ancl = Some (Anchor (fa,la) vm fresh))
+      (AS_OPT: (ver_code vins) # fresh = Some (Assume guard (fa,la) vm next))
+      (FS_SRC: (ver_code v) # ancl = Some (Anchor (fa,la) vm next))
+      (* (FINDF: find_base_version fa p = Some newver) *)
+      (UPDATE: update_regmap vm rm = OK newrm),
+      (match_states p v fid guard ancl params) Zero
+        (Halt_IR (v, ancl, rm), mkmut stk nil heap)
+        (Halt_IR (vins, fresh, rm), mkmut stk' nil heap)
+      
+| opt_match:           (* matching inside the optimized version *)
+    forall vins stk stk' heap lbl rm abs
+      (MATCHSTACK: (match_stack v fid guard ancl params) stk stk')
+      (OPT: insert_assume_version v fid guard ancl params = OK vins)
+      (DEFREGS: defined_regs_analysis (ver_code v) params (ver_entry v) = Some abs)
+      (DEF: defined rm (def_absstate_get lbl abs)),
+      (match_states p v fid guard ancl params) One
+        (Halt_IR (v, lbl, rm), mkmut stk nil heap)
+        (Halt_IR (vins, lbl, rm), mkmut stk' nil heap)
+                                        
+| refl_match:                   (* matching outside of the optimized version *)
+    forall synchro stk stk' top heap
+      (MATCHSTACK: (match_stack v fid guard ancl params) stk stk'),
+      (match_states p v fid guard ancl params) Zero (synchro, mkmut stk top heap) (synchro, mkmut stk' top heap).
+                                        
+(* | final_match:                  (* matching final states -> should be taken care of by refl*) *)
+(*     forall retval ms, *)
+(*       (match_states p v fid guard ancl params) One (Final retval ms) (Final retval ms). *)
+
+(** * Code preservation properties  *)
+Lemma code_preservation':
+  forall vsrc vins fid guard ancl lbl params,
+    insert_assume_version vsrc fid guard ancl params = OK vins ->
+    lbl <> ancl ->
+    forall iopt isrc,
+      (ver_code vins) # lbl = Some iopt ->
+      (ver_code vsrc) # lbl = Some isrc ->
+      iopt = isrc.
+Proof.
+  intros vsrc vins fid guard ancl lbl params OPT NOTFS iopt isrc CODEOPT CODESRC.
+  unfold insert_assume_version in OPT. repeat do_ok.
+  destruct (c!ancl) eqn:CODEFS; inv H1. destruct i; inv H0. repeat do_ok. destruct u.
+  simpl in CODEOPT. inv HDO.
+  poseq_destr (fresh_sug (Pos.succ ancl) (ver_code vsrc)) lbl.
+  - erewrite fresh_sug_correct in CODESRC; auto. inv CODESRC.
+  - rewrite PTree.gso in CODEOPT; auto. rewrite PTree.gso in CODEOPT; auto.
+    rewrite CODESRC in CODEOPT. inv CODEOPT. auto.
+Qed.
+
+Lemma safe_step_ir:
+  forall p rtl nc anc ms v pc rm,
+    safe (mixed_sem p rtl nc anc) (Halt_IR (v, pc, rm), ms) ->
+    exists t s', (mixed_step anc p rtl nc) (Halt_IR (v, pc, rm), ms) t s'.
+Proof.
+  intros p rtl nc anc ms v pc rm H. specialize (H (Halt_IR (v,pc,rm), ms) (star_refl _ _ _)).
+  destruct H as [[r FINAL]|[t [s'' STEP]]]; eauto. inv FINAL.
+Qed.
+
+Lemma safe_step:
+  forall p rtl nc anc synchro ms,
+    safe (mixed_sem p rtl nc anc) (synchro, ms) ->
+    (exists t s', (mixed_step anc p rtl nc) (synchro, ms) t s') \/ (exists r, synchro = EOE r).
+Proof.
+  intros p rtl nc anc synchro ms H.
+  specialize (H (synchro, ms) (star_refl _ _ _)). destruct H as [[r FINAL]|[t [s'' STEP]]]; eauto. inv FINAL.
+  right. eauto.
+Qed.
+
+Lemma step_code_ir:
+  forall p rtl nc anc v pc rm ms news t,
+    Step (mixed_sem p rtl nc anc) (Halt_IR (v, pc, rm), ms) t news ->
+    exists i, (ver_code v) ! pc = Some i.
+Proof.
+  intros. inv H; eauto.
+  unfold ir_step in STEP. repeat sdo_ok. unfold ir_int_step in HDO. repeat sdo_ok. eauto.
+Qed.
+
+
+Lemma safe_code:
+  forall p rtl nc anc s v pc rm ms top,
+    safe (mixed_sem p rtl nc anc) (Halt_IR (v, pc, rm), mkmut s top ms) ->
+    exists i, (ver_code v) ! pc = Some i.
+Proof.
+  intros. apply safe_step_ir in H as [s' [t STEP]].
+  eapply step_code_ir; simpl; eauto.
+Qed.
+
+
+Lemma code_preservation:        (* use at opt_match *)
+  forall p p' rtl nc s s' rm ms t news vsrc vins fid guard ancl lbl params,
+    insert_assume_version vsrc fid guard ancl params = OK vins ->
+    lbl <> ancl ->
+    safe (mixed_sem p rtl nc AnchorOn) (Halt_IR (vsrc, lbl, rm), mkmut s nil ms) ->
+    Step (mixed_sem p' rtl nc AnchorOn) (Halt_IR (vins, lbl, rm), mkmut s' nil ms) t news ->
+    (ver_code vsrc) # lbl = (ver_code vins) # lbl.
+Proof.
+  intros p p' rtl nc s s' rm ms t news vsrc vins fid guard ancl lbl params H H0 H1 H2.
+  apply safe_code in H1 as [isrc CODESRC]. apply step_code_ir in H2 as [iopt CODEOPT].
+  rewrite CODESRC. rewrite CODEOPT. f_equal. symmetry. eapply code_preservation'; eauto.
+Qed.
+
+(* The anchor instruction has been changed to point to the Assume *)
+Lemma anchor_changed:
+  forall vsrc fid guard vins ancl params,
+    insert_assume_version vsrc fid guard ancl params = OK vins ->
+    exists tgt vm fresh next,
+      (ver_code vins) # ancl = Some (Anchor tgt vm fresh) /\
+      (ver_code vsrc) # ancl = Some (Anchor tgt vm next) /\
+      (ver_code vins) # fresh = Some (Assume guard tgt vm next).
+Proof.
+  intros vsrc fid guard vins ancl params OPT. unfold insert_assume_version in OPT. repeat do_ok.
+  inv HDO. destruct ((ver_code vsrc)!ancl) eqn:FS_SRC; inv H1.
+  destruct i eqn:ANCHOR; inv H0. repeat do_ok. exists d. exists v.
+  exists (fresh_sug (Pos.succ ancl) (ver_code vsrc)). exists l. simpl.
+  split; auto; try split; auto. 
+  - poseq_destr (fresh_sug (Pos.succ ancl) (ver_code vsrc)) ancl.
+    + erewrite fresh_sug_correct in FS_SRC; eauto. inv FS_SRC.
+    + rewrite PTree.gso; auto. rewrite PTree.gss. auto.
+  - rewrite PTree.gss. auto.
+Qed.
+
+
+Lemma preservation_code:
+  forall vsrc vins fid guard ancl lbl params i,
+    insert_assume_version vsrc fid guard ancl params = OK vins ->
+    lbl <> ancl ->
+    (ver_code vsrc) # lbl = Some i ->
+    (ver_code vins) # lbl = Some i.
+Proof.
+  intros vsrc vins fid guard ancl lbl params i H H0 H1. unfold insert_assume_version in H. repeat do_ok.
+  destruct (c!ancl) eqn:CODEFS. 2: inv H2. destruct i0; inv H2. repeat do_ok. simpl. inv HDO.
+  rewrite PTree.gso. rewrite PTree.gso; auto. poseq_destr lbl (fresh_sug (Pos.succ ancl) (ver_code vsrc)); auto.
+  erewrite fresh_sug_correct in H1; auto. inv H1.
+Qed.
+  
+
+(** * Progress Preservation  *)
+Lemma evaluate_reg:
+  forall rm rs r,
+    defined rm (DefFlatRegset.Inj rs) ->
+    check_reg r rs = true ->
+    exists v, eval_reg r rm = OK v.
+Proof.
+  intros rm rs r H H0.
+  unfold check_reg in H0. rewrite PositiveSet.mem_spec in H0.
+  unfold defined in H. apply H in H0. destruct H0. exists x. unfold eval_reg. rewrite H0. auto.
+Qed.
+
+Lemma evaluate_expr:
+  forall rm rs e,
+    defined rm (DefFlatRegset.Inj rs) ->
+    check_expr e rs = true ->
+    exists v, eval_expr e rm = OK v.
+Proof.
+  intros rm rs e H H0. destruct e; simpl in H0.
+  - assert (H': exists v, eval_reg r rm = OK v /\ exists v0, eval_reg r0 rm = OK v0).
+    { destruct b; try solve[inv H0]; apply andb_prop in H0; destruct H0; eauto;
+        eapply evaluate_reg in H0; eapply evaluate_reg in H1; eauto; destruct H0; destruct H1; eauto. }
+    destruct H' as [v [EV [v' EV']]]. destruct b; simpl; rewrite EV; rewrite EV'; simpl; eauto.
+    inv H0.
+  - eapply evaluate_reg in H0; eauto. destruct H0. destruct u; simpl; rewrite H0; simpl; eauto.
+  - destruct z; simpl; eauto.
+Qed.
+
+Lemma base_version_set_version:
+  forall vins f,
+    base_version (set_version_function vins f) = base_version f.
+Proof.
+  intros vins f. unfold set_version_function, base_version. simpl. auto.
+Qed.
+
+Lemma current_version_set_version:
+  forall vins f,
+    current_version (set_version_function vins f) = vins.
+Proof.
+  intros vins f. unfold set_version_function, current_version. simpl. auto.
+Qed.
+
+
+
+
+(* Evaluating a guard if it uses defined registers should be defined *)
+(* Lemma evaluate_succeeds: *)
+(*   forall rm guard rs, *)
+(*     defined rm (DefFlatRegset.Inj rs) -> *)
+(*     check_guard guard rs = true -> *)
+(*     exists v, eval_list_expr guard rm v. *)
+(* Proof. *)
+(*   intros rm guard rs H H0. induction guard; intros. *)
+(*   - exists true. constructor. *)
+(*   - simpl in H0. apply andb_prop in H0. destruct H0. eapply evaluate_expr in H0; eauto. *)
+(*     destruct H0. destruct x. apply IHguard in H1. destruct H1. destruct z. *)
+(*     + esplit. eapply eval_cons_false; eauto. *)
+(*     + esplit. eapply eval_cons_true; eauto. unfold Zne. unfold not. intro. inv H1; inv H2. *)
+(*     + esplit. eapply eval_cons_true; eauto. unfold Zne. unfold not. intro. inv H1; inv H2. *)
+(* Qed. *)
+(* DEPRECATED until we use lists *)
+
+Ltac def_ok :=
+  match goal with
+  | [CODE: (ver_code ?vsrc) ! ?lbl = Some ?i |- _] =>
+    eapply def_analyze_correct; eauto; simpl; auto; unfold def_dr_transf; try rewrite CODE; auto
+  end.
+
+Lemma progress_preserved:
+  forall f vsrc vins fid guard ancl params s1 s2 p rtl nc i,
+    insert_assume_version vsrc fid guard ancl params = OK vins ->
+    find_function_ir fid p = Some f ->
+    vsrc = current_version f ->
+    match_states p vsrc fid guard ancl params i s1 s2 ->
+    safe (mixed_sem p rtl nc AnchorOn) s1 ->
+    (exists r : Integers.Int.int, final_mixed_state (set_version p fid vins) s2 r) \/
+    (exists (t : trace) (s2' : mixed_state),
+        Step (mixed_sem (set_version p fid vins) rtl nc AnchorOn) s2 t s2').
+Proof.
+  intros f vsrc vins fid guard ancl params s1 s2 p rtl nc i OPTV FINDOPT CURVER MATCH SAFE.
+  inv MATCH.
+  - unfold validator in VALIDATE. rewrite FS_SRC in VALIDATE. repeat do_ok.
+    destruct (def_absstate_get ancl d) eqn:ABSDR; inv H0.
+    destruct (check_expr guard r) eqn:CHECK; inv H1.
+    inv DEFREGS. rewrite ABSDR in DEF. eapply evaluate_expr in CHECK as [v EVAL]; eauto.
+    right. exists E0. rewrite OPT in OPTV. inv OPTV. destruct (bool_of_int v) eqn:BOOL.
+    + econstructor. apply IR_step. unfold ir_step. rewrite exec_bind2. unfold sbind2, sbind.
+      unfold ir_int_step. rewrite AS_OPT. simpl. rewrite exec_bind. unfold sbind, fret'.
+      rewrite EVAL. simpl. rewrite BOOL. simpl. eauto.
+    + econstructor. apply IR_step. unfold ir_step. rewrite exec_bind2. unfold sbind2, sbind.
+      unfold ir_int_step. rewrite AS_OPT. simpl. rewrite exec_bind. unfold sbind, fret'.
+      rewrite EVAL. simpl. rewrite BOOL. rewrite UPDATE. simpl. eauto.
+      
+  - poseq_destr lbl ancl.
+    + rewrite OPT in OPTV. inv OPTV. unfold insert_assume_version in OPT. repeat do_ok.
+      destruct (c!ancl) eqn:CODEFS; inv H1. destruct i; inv H0.
+      right. exists E0. exists (Halt_IR (vins, (fresh_sug (Pos.succ ancl) c), rm), mkmut stk' nil heap). 
+      repeat do_ok. simpl. destruct d as [ftgt ltgt].
+      apply safe_step_ir in SAFE as STEP. destruct STEP as [t [s'' STEP]].
+      inv HDO. inv STEP.
+      * exfalso. eapply ir_noanchor in STEP0; eauto.
+      * rewrite ANCHOR in CODEFS. inv CODEFS. eapply Anchor_go_on; eauto. simpl. rewrite PTree.gso.
+        rewrite PTree.gss. eauto. unfold not; intros H.
+        symmetry in H. apply fresh_sug_correct in H. rewrite H in ANCHOR. inv ANCHOR.
+      * rewrite ANCHOR in CODEFS. inv CODEFS. eapply Anchor_go_on; eauto. simpl. rewrite PTree.gso.
+        rewrite PTree.gss. eauto. unfold not; intros H.
+        symmetry in H. apply fresh_sug_correct in H. rewrite H in ANCHOR. inv ANCHOR.
+      
+    + apply safe_step_ir in SAFE as STEP. destruct STEP as [t [s'' STEP]].
+      right. rewrite OPT in OPTV. inv OPTV.
+      apply safe_code in SAFE. destruct SAFE as [i CODESRC].
+      eapply preservation_code in HEQ as SAME_CODE; eauto. 
+      inv STEP.
+      * exists t. unfold ir_step in STEP0. repeat sdo_ok. unfold ir_int_step in HDO.
+        rewrite CODESRC in HDO. repeat sdo_ok. inv HDO1.
+        { destruct i0; repeat sdo_ok.
+          - econstructor. eapply IR_step. unfold ir_step, ir_int_step. rewrite SAME_CODE. simpl. eauto.
+          - econstructor. eapply IR_step. unfold ir_step, ir_int_step. rewrite SAME_CODE. simpl.
+            unfold fret'. rewrite HDO. simpl. eauto.
+          - poseq_destr f0 fid.
+            + simpl in HDO. repeat sdo_ok.
+              econstructor. eapply IR_step. unfold ir_step, ir_int_step. rewrite SAME_CODE. simpl.
+              unfold sbind. unfold n_push_interpreter_stackframe. simpl. rewrite HDO. simpl. eauto.
+            + simpl in HDO. repeat sdo_ok.
+              econstructor. eapply IR_step. unfold ir_step, ir_int_step. rewrite SAME_CODE. simpl.
+              unfold sbind. unfold n_push_interpreter_stackframe. simpl. rewrite HDO. simpl. eauto.
+          - destruct (bool_of_int i) eqn:BOOL; repeat sdo_ok.
+            + econstructor. eapply IR_step. unfold ir_step, ir_int_step. rewrite SAME_CODE. simpl.
+              rewrite HDO1. simpl. rewrite BOOL. simpl. eauto.
+            + econstructor. eapply IR_step. unfold ir_step, ir_int_step. rewrite SAME_CODE. simpl.
+              rewrite HDO1. simpl. rewrite BOOL. simpl. eauto.
+          - econstructor. eapply IR_step. unfold ir_step, ir_int_step. rewrite SAME_CODE. simpl.
+            rewrite HDO. simpl. eauto.
+          - econstructor. eapply IR_step. unfold ir_step, ir_int_step. rewrite SAME_CODE. simpl.
+            rewrite HDO. simpl. eauto.
+          - econstructor. eapply IR_step. unfold ir_step, ir_int_step. rewrite SAME_CODE. simpl.
+            rewrite HDO1. simpl. rewrite HDO. simpl. unfold sbind. unfold n_memset in HDO2.
+            unfold n_memset. destruct (Integers.Int.lt i mem_size). inv HDO2. eauto. inv HDO2.
+          - econstructor. eapply IR_step. unfold ir_step, ir_int_step. rewrite SAME_CODE. simpl.
+            rewrite HDO. simpl. unfold sbind. unfold n_memget in HDO1.
+            unfold n_memget. destruct (Integers.Int.lt i mem_size). inv HDO1. 2: inv HDO1.
+            simpl. destruct (heap ! (intpos.pos_of_int i)); inv H0. eauto.
+          - destruct d. repeat sdo_ok. destruct (bool_of_int i) eqn:BOOL; repeat sdo_ok.
+            + econstructor. eapply IR_step. unfold ir_step, ir_int_step. rewrite SAME_CODE. simpl.
+              rewrite HDO1. simpl. rewrite BOOL. simpl. eauto.
+            + econstructor. eapply IR_step. unfold ir_step, ir_int_step. rewrite SAME_CODE. simpl.
+              rewrite HDO1. simpl. rewrite BOOL. simpl. rewrite HDO. simpl. eauto.
+          - destruct d. repeat sdo_ok. inv HDO. }
+
+      * exists E0. rewrite CODESRC in ANCHOR. inv ANCHOR.
+        exists (Halt_IR (vins, next, rm), mkmut stk' nil heap). eapply Anchor_go_on; eauto.
+      * exists E0. rewrite CODESRC in ANCHOR. inv ANCHOR.
+        exists (Halt_IR (vins, next, rm), mkmut stk' nil heap). eapply Anchor_go_on; eauto.
+                  
+  - apply safe_step in SAFE. destruct SAFE as [[t [s'' STEP]]| [r FINAL]].
+    2: { inv FINAL. left. exists r. constructor. }
+    right. inv STEP.
+    + destruct ms1. eapply addstk_same in STEP0 as [s [APP SAME]]; eauto.
+      2: apply addstk_irstep.
+      exists t. econstructor. eapply IR_step. simpl. eauto.
+    + destruct ms1. eapply addstk_same in STEP0 as [s [APP SAME]]; eauto.
+      2: apply addstk_asmstep.
+      exists t. econstructor. eapply x86_step. simpl. eauto.
+    + econstructor. econstructor. eapply rtl_step; eauto.
+    + destruct ms'. eapply addstk_same in BLOCK as [s [APP SAME]]; eauto.
+      2: { unfold block_step. repeat addstk_auto. unfold exec_block_instr. repeat addstk_auto.
+           unfold ASMinterpreter.prim_sem_dec. repeat addstk_auto. }
+      exists t. econstructor. eapply rtl_block_step. eauto.
+    + destruct ms2, ms3. eapply addstk_same in CALLEE as [s [APP SAME]]; eauto.
+      2: apply addstk_callee.
+      eapply addstk_prim_same in NOT_COMPILED as [stk2 [APP2 SAME2]]; try constructor.
+      apply app_same in APP2. subst.
+      eapply addstk_same in ARGS as [s3 [APP3 SAME3]]; eauto.
+      2: apply addstk_get_args.
+      poseq_destr fid fid0.
+      * econstructor. econstructor.
+        eapply Call_IR with (func:=set_version_function vins func) (ver:=vins); eauto.
+        unfold set_version, set_version_funlist. simpl. rewrite GETF. rewrite PTree.gss. auto.
+      * econstructor. econstructor.
+        eapply Call_IR; eauto. unfold set_version, set_version_funlist. simpl.
+        unfold find_function_ir in FINDOPT. rewrite FINDOPT. rewrite PTree.gso; auto.
+    + destruct ms2, ms3, ms4. eapply addstk_same in CALLEE as [s [APP SAME]]; eauto.
+      2: apply addstk_callee.
+      eapply addstk_prim_same in COMPILED as [stk2 [APP2 SAME2]]; try constructor.
+      apply app_same in APP2. subst.
+      eapply addstk_same in ARGS as [stk3 [APP3 SAME3]]. 2: apply addstk_set_args. subst.
+      eapply addstk_prim_same in LOAD as [stk4 [APP4 SAME4]]; try constructor. subst.
+      exists E0. econstructor. eapply Call_x86; eauto.
+    + destruct ms2, ms3. eapply addstk_same in CALLEE as [s [APP SAME]].
+      2: apply addstk_callee.
+      eapply addstk_prim_same in COMPILED as [stk2 [APP2 SAME2]]; try constructor.
+      apply app_same in APP2. subst.
+      eapply addstk_same in ARGS as [stk3 [APP3 SAME3]]. 2: apply addstk_set_args. subst.
+      econstructor. econstructor. eapply Call_RTL; eauto.
+    + destruct ms1, ms2. eapply addstk_same in CALLEE as [s [APP SAME]].
+      2: apply addstk_callee.
+      eapply addstk_prim_same in COMPILED as [stk2 [APP2 SAME2]]; try constructor.
+      apply app_same in APP2. subst.
+      eapply addstk_same in ARGS as [stk3 [APP3 SAME3]]. 2: apply addstk_set_args. subst.
+      econstructor. econstructor. eapply Call_RTL_Block; eauto.
+    + destruct ms1. unfold jit.get_retval in RETVAL. destruct loc eqn:LOC.
+      * destruct top eqn:TOP; inv RETVAL.
+        simpl in OPEN_SF. unfold n_open_stackframe in OPEN_SF. simpl in OPEN_SF.
+        destruct state_stacktop; inv OPEN_SF.
+        inv MATCHSTACK; inv H0. destruct sf; inv H1.
+        2: { destruct a, p, p0, p. inv H0. }
+        inv MSF.
+        ** econstructor. econstructor. eapply Return_IR; eauto.
+           simpl. unfold sbind. simpl. eauto.
+           simpl. unfold n_open_stackframe. simpl. eauto.
+        ** econstructor. econstructor. eapply Return_IR; eauto.
+           simpl. unfold sbind. simpl. eauto.
+           simpl. unfold n_open_stackframe. simpl. eauto.
+      * inv RETVAL.
+        simpl in OPEN_SF. unfold n_open_stackframe in OPEN_SF. simpl in OPEN_SF.
+        destruct state_stacktop; inv OPEN_SF.
+        inv MATCHSTACK; inv H0. destruct sf; inv H1.
+        2: { destruct a, p, p0, p. inv H0. }
+        inv MSF.
+        ** econstructor. econstructor. eapply Return_IR; eauto.
+           simpl. unfold sbind. simpl. eauto.
+           simpl. unfold n_open_stackframe. simpl. eauto.
+        ** econstructor. econstructor. eapply Return_IR; eauto.
+           simpl. unfold sbind. simpl. eauto.
+           simpl. unfold n_open_stackframe. simpl. eauto.
+    + destruct loc.
+      * simpl in RETVAL.  repeat sdo_ok.  unfold n_load in HDO. simpl in HDO.
+        destruct top; inv HDO.
+        simpl in OPEN_SF. unfold n_open_stackframe in OPEN_SF. simpl in OPEN_SF.
+        destruct top; inv OPEN_SF. destruct stk; inv H0. destruct s; inv H1.
+        destruct a, p, p0, p. inv H0. inv MATCHSTACK. inv MSF.
+        simpl in SET_RETVAL. unfold n_save in SET_RETVAL. inv SET_RETVAL.
+        simpl in LOAD_CONT. repeat sdo_ok. unfold n_load_prog_code in HDO. simpl in HDO.
+        destruct (nc ! (intpos.pos_of_int caller_fid)) eqn:LOADC; inv HDO.
+        destruct a. simpl in LOAD_CONT.
+        destruct (t ! (intpos.pos_of_int cont_lbl)) eqn:LOAD; inv LOAD_CONT.
+        econstructor. econstructor. eapply Return_x86.
+        ** simpl. unfold sbind. unfold n_load. simpl. eauto.
+        ** simpl. unfold n_open_stackframe. simpl. eauto.
+        ** simpl. unfold n_save. simpl. eauto.
+        ** simpl. unfold sbind. unfold n_load_prog_code. simpl. rewrite LOADC. simpl. rewrite LOAD. eauto.
+        ** eauto.
+      * inv RETVAL. simpl in OPEN_SF. unfold n_open_stackframe in OPEN_SF. simpl in OPEN_SF.
+        destruct top; inv OPEN_SF. destruct stk; inv H0. destruct s; inv H1.
+        destruct a, p, p0, p. inv H0. inv MATCHSTACK. inv MSF.
+        simpl in SET_RETVAL. unfold n_save in SET_RETVAL. inv SET_RETVAL.
+        simpl in LOAD_CONT. repeat sdo_ok. unfold n_load_prog_code in HDO. simpl in HDO.
+        destruct (nc ! (intpos.pos_of_int caller_fid)) eqn:LOADC; inv HDO.
+        destruct a. simpl in LOAD_CONT.
+        destruct (t ! (intpos.pos_of_int cont_lbl)) eqn:LOAD; inv LOAD_CONT.
+        econstructor. econstructor. eapply Return_x86.
+        ** simpl. auto.
+        ** simpl. unfold n_open_stackframe. simpl. eauto.
+        ** simpl. unfold n_save. simpl. eauto.
+        ** simpl. unfold sbind. unfold n_load_prog_code. simpl. rewrite LOADC. simpl. rewrite LOAD. eauto.
+        ** eauto.
+    + destruct loc.
+      * destruct top; inv RETVAL. inv OPEN_SF. unfold n_open_stackframe in H0. simpl in H0.
+        destruct top; inv H0. destruct stk; inv H1. destruct s; inv H0.
+        destruct a, p, p0, p; inv H1. simpl in SETRETVAL. unfold n_save in SETRETVAL. inv SETRETVAL.
+        simpl in NOT_COMPILED. unfold n_check_compiled in NOT_COMPILED. simpl in NOT_COMPILED.
+        destruct (nc ! fid0) eqn:NOT; inv NOT_COMPILED.
+        inv MATCHSTACK. inv MSF.
+        econstructor. econstructor. eapply Return_RTL; eauto.
+        ** simpl. unfold sbind. simpl. eauto.
+        ** simpl. unfold n_open_stackframe. simpl. eauto.
+        ** simpl. unfold n_save. simpl. eauto.
+        ** simpl. unfold n_check_compiled. simpl. rewrite NOT. auto.
+      * inv RETVAL. inv OPEN_SF. unfold n_open_stackframe in H0. simpl in H0.
+        destruct top; inv H0. destruct stk; inv H1. destruct s; inv H0.
+        destruct a, p, p0, p; inv H1. simpl in SETRETVAL. unfold n_save in SETRETVAL. inv SETRETVAL.
+        simpl in NOT_COMPILED. unfold n_check_compiled in NOT_COMPILED. simpl in NOT_COMPILED.
+        destruct (nc ! fid0) eqn:NOT; inv NOT_COMPILED.
+        inv MATCHSTACK. inv MSF.
+        econstructor. econstructor. eapply Return_RTL; simpl; eauto.
+        ** unfold n_open_stackframe. simpl. eauto.
+        ** unfold n_save. simpl. eauto.
+        ** unfold n_check_compiled. simpl. rewrite NOT. auto.
+    + destruct loc.
+      * destruct top; inv RETVAL. inv OPEN_SF. unfold n_open_stackframe in H0. simpl in H0.
+        destruct top; inv H0. destruct stk; inv H1. destruct s; inv H0.
+        destruct a, p, p0, p; inv H1. simpl in SETRETVAL. unfold n_save in SETRETVAL. inv SETRETVAL.
+        simpl in NOT_COMPILED. unfold n_check_compiled in NOT_COMPILED. simpl in NOT_COMPILED.
+        destruct (nc ! fid0) eqn:NOT; inv NOT_COMPILED.
+        inv MATCHSTACK. inv MSF.
+        econstructor. econstructor. eapply Return_RTL_Block; eauto.
+        ** simpl. unfold sbind. simpl. eauto.
+        ** simpl. unfold n_open_stackframe. simpl. eauto.
+        ** simpl. unfold n_save. simpl. eauto.
+        ** simpl. unfold n_check_compiled. simpl. rewrite NOT. auto.
+      * inv RETVAL. inv OPEN_SF. unfold n_open_stackframe in H0. simpl in H0.
+        destruct top; inv H0. destruct stk; inv H1. destruct s; inv H0.
+        destruct a, p, p0, p; inv H1. simpl in SETRETVAL. unfold n_save in SETRETVAL. inv SETRETVAL.
+        simpl in NOT_COMPILED. unfold n_check_compiled in NOT_COMPILED. simpl in NOT_COMPILED.
+        destruct (nc ! fid0) eqn:NOT; inv NOT_COMPILED.
+        inv MATCHSTACK. inv MSF.
+        econstructor. econstructor. eapply Return_RTL_Block; simpl; eauto.
+         ** unfold n_open_stackframe. simpl. eauto.
+         ** unfold n_save. simpl. eauto.
+         ** unfold n_check_compiled. simpl. rewrite NOT. auto.
+    + destruct loc.
+      * destruct top; inv RETVAL. inv OPEN_SF. unfold n_open_stackframe in H0. simpl in H0.
+        destruct top; inv H0. destruct stk; inv H1.
+        2: { destruct s; inv H0. destruct a, p, p0, p; inv H1. }
+        inv MATCHSTACK. econstructor. econstructor. eapply Return_EOE; eauto.
+        simpl. unfold sbind. simpl. eauto.
+        simpl. unfold n_open_stackframe. simpl. eauto.
+      * inv RETVAL. inv OPEN_SF. unfold n_open_stackframe in H0. simpl in H0.
+        destruct top; inv H0. destruct stk; inv H1.
+        2: { destruct s; inv H0. destruct a, p, p0, p; inv H1. }
+        inv MATCHSTACK. econstructor. econstructor. eapply Return_EOE; eauto.
+        simpl. unfold sbind. simpl. eauto.
+        simpl. unfold n_open_stackframe. simpl. eauto.
+    + destruct ms1, ms2. eapply addstk_same in TARGET as [s [APP SAME]].
+      2: apply addstk_target.
+      eapply addstk_same in BUILD_RM as [s2 [APP2 SAME2]].
+      2: apply addstk_build.
+      poseq_destr fid ftgt.
+      * econstructor. econstructor. eapply Deopt; eauto.
+        unfold set_version, set_version_funlist. simpl. unfold find_function_ir in FINDOPT. rewrite FINDOPT.
+        rewrite PTree.gss; auto.
+      * econstructor. econstructor. eapply Deopt; eauto.
+        unfold set_version, set_version_funlist. simpl. unfold find_function_ir in FINDOPT. rewrite FINDOPT.
+        rewrite PTree.gso; eauto.
+    + destruct ms1. eapply addstk_same in PRIM_CALL as [s [APP SAME]].
+      2: { unfold ASMinterpreter.prim_sem_dec. repeat addstk_auto. }
+      econstructor. econstructor. eapply RTL_prim; eauto.
+    + econstructor. econstructor. eapply RTL_end; eauto.
+    + econstructor. econstructor. eapply RTL_block_end; eauto.
+    + econstructor. econstructor. eapply Anchor_go_on; eauto.
+    + econstructor. econstructor. eapply Anchor_deopt; eauto.
+Qed.
+
+(** * The Internal Backward Simulation  *)
+Theorem assume_insertion_correct:
+  forall p rtl nc fid guard fs_lbl newp,
+    insert_assume fid guard fs_lbl p = OK newp ->
+    backward_internal_simulation p newp rtl rtl nc nc AnchorOn AnchorOn.
+Proof.
+  intros p rtl nc fid guard fs_lbl newp OPT. unfold insert_assume in OPT. repeat do_ok.
+  rename HDO1 into FINDOPTF. rename v into vins. set (vsrc:=current_version f).
+  assert (OPTV: insert_assume_version vsrc fid guard fs_lbl (fn_params f) = OK vins) by auto.
+  unfold insert_assume_version in HDO0. repeat do_ok. inv HDO. destruct u.
+  set (c:=ver_code vsrc).  rename HDO0 into VALIDATE. fold vsrc in VALIDATE.
+  fold vsrc in H1. fold c in H1. destruct (c!fs_lbl) eqn:CODE_FS; inv H1.
+  destruct i; inv H0. repeat do_ok. rename d into tgt. rename v into vm_fs. rename l into next_fs.
+  rename HDO0 into CODE_NEXT.
+  set (vins := {| ver_code := (c # fs_lbl <- (Anchor tgt vm_fs (fresh_sug (Pos.succ fs_lbl) c))) #  (fresh_sug (Pos.succ fs_lbl) c) <- (Assume guard tgt vm_fs next_fs); ver_entry := ver_entry vsrc |}). fold vins in OPTV.
+  apply Backward_internal_simulation with (bsim_order:=as_order) (bsim_match_states:=match_states p vsrc fid guard fs_lbl (fn_params f)).
+  - apply wfounded.
+  - unfold call_refl. unfold p_reflexive. intros s H. inv H. exists Zero. destruct ms. apply refl_match.
+    apply match_stack_same.
+
+  - intros. inv H1. inv H. econstructor. split. apply star_refl. constructor.
+
+  - intros. eapply progress_preserved; eauto. 
+
+  - intros s2 t s2' STEP i0 s1 MATCH SAFE.
+    inv MATCH.
+
+    + rewrite OPT in OPTV. inv OPTV. (* assume_match *)
+      inv STEP.
+      2: { rewrite ANCHOR in AS_OPT. inv AS_OPT. }
+      2: { rewrite ANCHOR in AS_OPT. inv AS_OPT. }
+      simpl in STEP0. unfold ir_step, ir_int_step in STEP0.
+      rewrite AS_OPT in STEP0. simpl in STEP0. repeat sdo_ok.
+      destruct (bool_of_int i0) eqn:GUARD. inv HDO.
+      * exists One. econstructor. split.    (* Assume holds *)
+        ** left. apply plus_one. eapply Anchor_go_on; eauto.
+        ** simpl. eapply opt_match; eauto.
+           eapply def_analyze_correct; eauto. simpl; auto. unfold def_dr_transf. rewrite FS_SRC. auto.
+      * repeat sdo_ok. exists Zero. econstructor. split. (* Assume fails *)
+        ** left. apply plus_one. eapply Anchor_deopt; eauto.
+        ** simpl. eapply refl_match. auto.
+        
+    + rewrite OPT in OPTV. inv OPTV. (* opt_match *)
+      poseq_destr lbl fs_lbl.
+      (* We are at the anchor used for insertion*)
+      { assert (OPT': insert_assume_version vsrc fid guard fs_lbl (fn_params f)= OK vins) by auto.
+        apply anchor_changed in OPT as [[fa la][vm [fresh [next [CODE_INS_FS [CODE_SRC_FS CODE_INS_AS]]]]]].
+        unfold c in CODE_FS. rewrite CODE_FS in CODE_SRC_FS. inv CODE_SRC_FS. inv STEP.
+        - unfold ir_step, ir_int_step in STEP0. rewrite CODE_INS_FS in STEP0. simpl in STEP0. inv STEP0.
+        - rewrite ANCHOR in CODE_INS_FS. inv CODE_INS_FS.
+        (* The Anchor goes on in OPT. In SRC, it will depend on how the Assume evaluates *)
+        (* So we take a stuttering step in the SRC *)
+          exists Zero. econstructor. split.
+          + right. split. apply star_refl. constructor.
+          + eapply assume_match; eauto.
+        - rewrite ANCHOR in CODE_INS_FS. inv CODE_INS_FS.
+        (* The Anchor deopts in both OPT and SRC *)
+          exists Zero. econstructor. split.
+          + left. apply plus_one. eapply Anchor_deopt; eauto.
+          + eapply refl_match; eauto. }
+      
+      (* We are not at the Anchor used for insertion *)
+      { eapply code_preservation in OPT as SAME_CODE; eauto.
+        inv STEP.
+        - unfold ir_step, ir_int_step in STEP0. repeat sdo_ok. destruct p0 as [t it].
+          destruct i0; repeat sdo_ok.
+          + exists One. econstructor. split.
+            * left. apply plus_one. eapply IR_step. unfold ir_step, ir_int_step.
+              rewrite SAME_CODE. simpl. eauto.
+            * simpl. eapply opt_match; eauto. def_ok. rewrite SAME_CODE. auto.
+          + exists One. econstructor. split.
+            * left. apply plus_one. eapply IR_step. unfold ir_step, ir_int_step.
+              rewrite SAME_CODE. simpl. rewrite HDO. simpl. eauto.
+            * eapply opt_match; eauto. def_ok. rewrite SAME_CODE. auto.
+
+          + simpl in HDO. repeat sdo_ok. unfold n_push_interpreter_stackframe in HDO0.
+            simpl in HDO0. inv HDO0.
+            exists Zero. econstructor. split.
+            * left. apply plus_one. eapply IR_step; eauto. unfold ir_step, ir_int_step.
+              rewrite SAME_CODE. simpl. unfold sbind. unfold n_push_interpreter_stackframe.
+              simpl. rewrite HDO. simpl. eauto.
+            * simpl. eapply refl_match; eauto. constructor; auto.
+              eapply frame_opt; eauto. intros. def_ok. rewrite SAME_CODE. apply define_insert. auto.
+          + destruct (bool_of_int i0) eqn:BOOL; repeat sdo_ok.
+            * exists One. econstructor. split.
+              ** left. apply plus_one. eapply IR_step. unfold ir_step, ir_int_step.
+                 rewrite SAME_CODE. simpl. rewrite HDO2. simpl. rewrite BOOL. simpl. eauto.
+              ** eapply opt_match; eauto. def_ok. rewrite SAME_CODE. auto.
+            * exists One. econstructor. split.
+              ** left. apply plus_one. eapply IR_step. unfold ir_step, ir_int_step.
+                 rewrite SAME_CODE. simpl. rewrite HDO2. simpl. rewrite BOOL. simpl. eauto.
+              ** eapply opt_match; eauto. def_ok. rewrite SAME_CODE. auto.
+          + exists Zero. econstructor. split.
+            * left. apply plus_one. eapply IR_step. unfold ir_step, ir_int_step.
+              rewrite SAME_CODE. simpl. rewrite HDO. simpl. eauto.
+            * simpl. eapply refl_match; eauto.
+          + exists One. econstructor. split.
+            * left. apply plus_one. eapply IR_step. unfold ir_step, ir_int_step.
+              rewrite SAME_CODE. simpl. rewrite HDO. simpl. eauto.
+            * eapply opt_match; eauto. def_ok. rewrite SAME_CODE. apply define_insert. auto.
+          + unfold n_memset in HDO3. destruct (Integers.Int.lt i0 mem_size) eqn:RANGE; inv HDO3.
+            exists One. econstructor. split.
+            * left. apply plus_one. eapply IR_step. unfold ir_step, ir_int_step.
+              rewrite SAME_CODE. simpl. rewrite HDO. simpl. rewrite HDO2. simpl.
+              unfold n_memset. rewrite RANGE. unfold sbind. simpl. eauto.
+            * eapply opt_match; eauto. def_ok. rewrite SAME_CODE. auto.
+          + unfold n_memget in HDO2. destruct (Integers.Int.lt i0 mem_size) eqn:RANGE; inv HDO2.
+            destruct (heap ! (intpos.pos_of_int i0)) eqn:HEAP; inv H0.
+            exists One. econstructor. split.
+            * left. apply plus_one. eapply IR_step. unfold ir_step, ir_int_step.
+              rewrite SAME_CODE. simpl. rewrite HDO. simpl. 
+              unfold n_memget. rewrite RANGE. unfold sbind. simpl. rewrite HEAP. eauto.
+            * eapply opt_match; eauto. def_ok. rewrite SAME_CODE. apply define_insert. auto.
+          + destruct d. repeat sdo_ok. destruct (bool_of_int i0) eqn:BOOL; repeat sdo_ok.
+            * exists One. econstructor. split.
+              ** left. apply plus_one. eapply IR_step. unfold ir_step, ir_int_step.
+                 rewrite SAME_CODE. simpl. rewrite HDO2. simpl. rewrite BOOL. simpl. eauto.
+              ** eapply opt_match; eauto. def_ok. rewrite SAME_CODE. auto.
+            * exists Zero. econstructor. split.
+              ** left. apply plus_one. eapply IR_step. unfold ir_step, ir_int_step.
+                 rewrite SAME_CODE. simpl. rewrite HDO2. simpl. rewrite BOOL. rewrite HDO. simpl. eauto.
+              ** simpl. eapply refl_match; eauto.
+          + destruct d. inv HDO.
+        
+        - exists One. econstructor. split.
+          + left. apply plus_one. eapply Anchor_go_on; eauto. rewrite SAME_CODE. apply ANCHOR.
+          + eapply opt_match; eauto. clear CODE_NEXT CODE_FS. def_ok. rewrite ANCHOR in SAME_CODE.
+            eauto. simpl; auto. rewrite SAME_CODE. rewrite ANCHOR. auto.
+        - exists Zero. econstructor. split.
+          + left. apply plus_one. eapply Anchor_deopt; eauto. rewrite SAME_CODE. eauto.
+          + eapply refl_match. auto.
+      }
+            
+
+    + { inv STEP.                 (* refl_match *)
+        - destruct ms1. eapply addstk_same in STEP0 as [s [APP SAME]]; eauto.
+          2: apply addstk_irstep.
+          exists Zero. econstructor. split.
+          + left. apply plus_one. eapply IR_step; eauto.
+          + apply refl_match. subst. apply app_match; auto. apply match_stack_same.
+        - destruct ms1. eapply addstk_same in STEP0 as [s [APP SAME]]; eauto.
+          2: apply addstk_asmstep.
+          exists Zero. econstructor. split.
+          + left. apply plus_one. eapply x86_step; eauto.
+          + apply refl_match. subst. apply app_match; auto. apply match_stack_same.
+        - exists Zero. econstructor. split.
+          + left. apply plus_one. eapply rtl_step; eauto.
+          + apply refl_match; auto.
+        - destruct ms'. eapply addstk_same in BLOCK as [s [APP SAME]]; eauto.
+          2: { unfold block_step. repeat addstk_auto. unfold exec_block_instr. repeat addstk_auto.
+               unfold ASMinterpreter.prim_sem_dec. repeat addstk_auto. }
+          exists Zero. econstructor. split.
+          + left. apply plus_one. eapply rtl_block_step; eauto.
+          + apply refl_match. subst. apply app_match; auto. apply match_stack_same.
+        - unfold find_function_ir in FINDOPTF.
+          unfold set_version, set_version_funlist in GETF. simpl in GETF. rewrite FINDOPTF in GETF.
+          poseq_destr fid fid0.
+          +                     (* Calling the optimized function *)
+            destruct ms2. eapply addstk_same in CALLEE as [s [APP SAME]].
+            2: apply addstk_callee.
+            simpl in NOT_COMPILED. unfold n_check_compiled in NOT_COMPILED. simpl in NOT_COMPILED.
+            destruct (nc!fid0) eqn:NOT; inv NOT_COMPILED.
+            destruct ms3. eapply addstk_same in ARGS as [s2 [APP2 SAME2]].
+            rewrite PTree.gss in GETF. inv GETF.
+            2: apply addstk_get_args.
+            exists One. econstructor. split.
+            * left. apply plus_one. eapply Call_IR; eauto; simpl.
+              ** unfold n_check_compiled. simpl. rewrite NOT. eauto.
+            * simpl.  rewrite current_version_set_version. unfold vsrc.
+              (* eapply opt_match. *) admit.
+              (* we need to add to the semantics that the top is empty *)
+          +   (* calling another function *)
+            rewrite PTree.gso in GETF; auto.
+            destruct ms2. eapply addstk_same in CALLEE as [s [APP SAME]].
+            2: apply addstk_callee.
+            simpl in NOT_COMPILED. unfold n_check_compiled in NOT_COMPILED. simpl in NOT_COMPILED.
+            destruct (nc!fid0) eqn:NOT; inv NOT_COMPILED.
+            destruct ms3. eapply addstk_same in ARGS as [s2 [APP2 SAME2]].
+            2: apply addstk_get_args.
+            exists Zero. econstructor. split.
+            * left. apply plus_one. eapply Call_IR; eauto; simpl.
+              ** unfold n_check_compiled. simpl. rewrite NOT. eauto.
+            * eapply refl_match. subst. apply match_app. apply match_app. auto.
+        - destruct loc.
+          + simpl in CALLEE. repeat sdo_ok. unfold n_load in HDO. simpl in HDO. destruct top; inv HDO.
+            simpl in COMPILED. unfold n_check_compiled in COMPILED. simpl in COMPILED.
+            destruct (nc ! (intpos.pos_of_int i0)) eqn:COMP; inv COMPILED.
+            destruct ms3. eapply addstk_same in ARGS as [s [APP SAME]]; eauto.
+            2: apply addstk_set_args.
+            simpl in LOAD. repeat sdo_ok. unfold n_load_prog_code in HDO. simpl in HDO.
+            rewrite COMP in HDO. inv HDO.
+            exists Zero. econstructor. split.
+            * left. apply plus_one. eapply Call_x86; eauto; simpl.
+              ** unfold n_load, sbind. simpl. eauto.
+              ** unfold n_check_compiled. simpl. rewrite COMP. eauto.
+              ** unfold n_load_prog_code, sbind. simpl. rewrite COMP. eauto.
+            * eapply refl_match. apply app_match; auto. apply match_stack_same.
+          + simpl in CALLEE. inv CALLEE.
+            simpl in COMPILED. unfold n_check_compiled in COMPILED. simpl in COMPILED.
+            destruct (nc ! fid0) eqn:COMP; inv COMPILED.
+            destruct ms3. eapply addstk_same in ARGS as [s [APP SAME]]; eauto.
+            2: apply addstk_set_args.
+            simpl in LOAD. repeat sdo_ok. unfold n_load_prog_code in HDO. simpl in HDO.
+            rewrite COMP in HDO. inv HDO.
+            exists Zero. econstructor. split.
+            * left. apply plus_one. eapply Call_x86; eauto; simpl.
+              ** unfold n_load, sbind. simpl. eauto.
+              ** unfold n_check_compiled. simpl. rewrite COMP. eauto.
+              ** unfold n_load_prog_code, sbind. simpl. rewrite COMP. eauto.
+            * eapply refl_match. apply app_match; auto. apply match_stack_same.
+        - destruct loc.
+          + simpl in CALLEE. repeat sdo_ok. unfold n_load in HDO. simpl in HDO. destruct top; inv HDO.
+            simpl in COMPILED. unfold n_check_compiled in COMPILED. simpl in COMPILED.
+            destruct (nc ! (intpos.pos_of_int i0)) eqn:COMP; inv COMPILED.
+            destruct ms3. eapply addstk_same in ARGS as [s [APP SAME]]; eauto.
+            2: apply addstk_set_args.
+            exists Zero. econstructor. split.
+            * left. apply plus_one. eapply Call_RTL; eauto; simpl.
+              ** unfold n_load, sbind. simpl. eauto.
+              ** unfold n_check_compiled. simpl. rewrite COMP. eauto.
+            * eapply refl_match. subst. apply app_match; auto. apply match_stack_same.
+          + simpl in CALLEE. inv CALLEE.
+            simpl in COMPILED. unfold n_check_compiled in COMPILED. simpl in COMPILED.
+            destruct (nc ! fid0) eqn:COMP; inv COMPILED.
+            destruct ms3. eapply addstk_same in ARGS as [s [APP SAME]]; eauto.
+            2: apply addstk_set_args.
+            exists Zero. econstructor. split.
+            * left. apply plus_one. eapply Call_RTL; eauto; simpl.
+              ** unfold n_load, sbind. simpl. eauto.
+              ** unfold n_check_compiled. simpl. rewrite COMP. eauto.
+            * eapply refl_match. subst. apply app_match; auto. apply match_stack_same.
+        - destruct loc.
+          + simpl in CALLEE. repeat sdo_ok. unfold n_load in HDO. simpl in HDO. destruct top; inv HDO.
+            simpl in COMPILED. unfold n_check_compiled in COMPILED. simpl in COMPILED.
+            destruct (nc ! (intpos.pos_of_int i0)) eqn:COMP; inv COMPILED.
+            destruct ms2. eapply addstk_same in ARGS as [s [APP SAME]]; eauto.
+            2: apply addstk_set_args.
+            exists Zero. econstructor. split.
+            * left. apply plus_one. eapply Call_RTL_Block; eauto; simpl.
+              ** unfold n_load, sbind. simpl. eauto.
+              ** unfold n_check_compiled. simpl. rewrite COMP. eauto.
+            * eapply refl_match. subst. apply app_match; auto. apply match_stack_same.
+          + simpl in CALLEE. inv CALLEE.
+            simpl in COMPILED. unfold n_check_compiled in COMPILED. simpl in COMPILED.
+            destruct (nc ! fid0) eqn:COMP; inv COMPILED.
+            destruct ms2. eapply addstk_same in ARGS as [s [APP SAME]]; eauto.
+            2: apply addstk_set_args.
+            exists Zero. econstructor. split.
+            * left. apply plus_one. eapply Call_RTL_Block; eauto; simpl.
+              ** unfold n_load, sbind. simpl. eauto.
+              ** unfold n_check_compiled. simpl. rewrite COMP. eauto.
+            * eapply refl_match. subst. apply app_match; auto. apply match_stack_same.
+        - destruct loc.
+          + simpl in RETVAL; repeat sdo_ok. unfold n_load in HDO. simpl in HDO. destruct top; inv HDO.
+            simpl in OPEN_SF. unfold n_open_stackframe in OPEN_SF. simpl in OPEN_SF.
+            destruct top; inv OPEN_SF. destruct stk'; inv H0. destruct s; inv H1.
+            2: { destruct a,p,p0,p. inv H0. }
+            inv MATCHSTACK. inv MSF.
+            * exists Zero. econstructor. split. (* Returning to the same function *)
+              ** left. apply plus_one. eapply Return_IR; eauto.
+                 *** simpl. unfold n_load, sbind. simpl. eauto.
+                 *** simpl. unfold n_open_stackframe. simpl. eauto.
+              ** eapply refl_match; eauto.
+            * exists One. econstructor. split. (* Returning to the optimized IR *)
+              ** left. apply plus_one. eapply Return_IR; eauto.
+                 *** simpl. unfold n_load, sbind. simpl. eauto.
+                 *** simpl. unfold n_open_stackframe. simpl. eauto.
+              ** eapply opt_match; eauto.
+          + simpl in RETVAL. inv RETVAL.
+            simpl in OPEN_SF. unfold n_open_stackframe in OPEN_SF. simpl in OPEN_SF.
+            destruct top; inv OPEN_SF. destruct stk'; inv H0. destruct s; inv H1.
+            2: { destruct a,p,p0,p. inv H0. }
+            inv MATCHSTACK. inv MSF.
+            * exists Zero. econstructor. split. (* Returning to the same function *)
+              ** left. apply plus_one. eapply Return_IR; eauto.
+                 *** simpl. eauto.
+                 *** simpl. unfold n_open_stackframe. simpl. eauto.
+              ** eapply refl_match; eauto.
+            * exists One. econstructor. split. (* Returning to the optimized IR *)
+              ** left. apply plus_one. eapply Return_IR; eauto.
+                 *** simpl. eauto.
+                 *** simpl. unfold n_open_stackframe. simpl. eauto.
+              ** eapply opt_match; eauto.
+        - destruct loc.
+          + simpl in RETVAL. repeat sdo_ok. unfold n_load in HDO. simpl in HDO. destruct top; inv HDO.
+            simpl in OPEN_SF. unfold n_open_stackframe in OPEN_SF. simpl in OPEN_SF.
+            destruct top; inv OPEN_SF. destruct stk'; inv H0. destruct s; inv H1. destruct a, p, p0, p.
+            inv H0. simpl in SET_RETVAL. unfold n_save in SET_RETVAL. simpl in SET_RETVAL. inv SET_RETVAL.
+            simpl in LOAD_CONT. repeat sdo_ok. destruct a.
+            unfold n_load_prog_code in HDO. simpl in HDO. destruct (nc!(intpos.pos_of_int caller_fid)) eqn:LOAD; inv HDO.
+            simpl in LOAD_CONT.
+            destruct (t!(intpos.pos_of_int cont_lbl)) eqn:LOAD2; inv LOAD_CONT.
+            inv MATCHSTACK. inv MSF.
+            exists Zero. econstructor. split.
+            * left. apply plus_one. eapply Return_x86; eauto; simpl.
+              ** unfold n_load, sbind. simpl. eauto.
+              ** unfold n_open_stackframe. simpl. eauto.
+              ** unfold n_save. simpl. eauto.
+              ** unfold n_load_prog_code, sbind. simpl.  rewrite LOAD. simpl. rewrite LOAD2. eauto.
+            * eapply refl_match. auto.
+          + simpl in RETVAL. inv RETVAL.
+            simpl in OPEN_SF. unfold n_open_stackframe in OPEN_SF. simpl in OPEN_SF.
+            destruct top; inv OPEN_SF. destruct stk'; inv H0. destruct s; inv H1. destruct a, p, p0, p.
+            inv H0. simpl in SET_RETVAL. unfold n_save in SET_RETVAL. simpl in SET_RETVAL. inv SET_RETVAL.
+            simpl in LOAD_CONT. repeat sdo_ok. destruct a.
+            unfold n_load_prog_code in HDO. simpl in HDO. destruct (nc!(intpos.pos_of_int caller_fid)) eqn:LOAD; inv HDO.
+            simpl in LOAD_CONT.
+            destruct (t!(intpos.pos_of_int cont_lbl)) eqn:LOAD2; inv LOAD_CONT.
+            inv MATCHSTACK. inv MSF.
+            exists Zero. econstructor. split.
+            * left. apply plus_one. eapply Return_x86; eauto; simpl.
+              ** unfold n_load, sbind. simpl. eauto.
+              ** unfold n_open_stackframe. simpl. eauto.
+              ** unfold n_save. simpl. eauto.
+              ** unfold n_load_prog_code, sbind. simpl.  rewrite LOAD. simpl. rewrite LOAD2. eauto.
+            * eapply refl_match. auto.
+        - destruct loc.
+          + simpl in RETVAL. repeat sdo_ok. unfold n_load in HDO. simpl in HDO. destruct top; inv HDO.
+            simpl in OPEN_SF. unfold n_open_stackframe in OPEN_SF. simpl in OPEN_SF.
+            destruct top; inv OPEN_SF. destruct stk'; inv H0. destruct s; inv H1. destruct a, p, p0, p.
+            inv H0. simpl in SETRETVAL. unfold n_save in SETRETVAL. simpl in SETRETVAL. inv SETRETVAL.
+            simpl in NOT_COMPILED. unfold n_check_compiled in NOT_COMPILED. simpl in NOT_COMPILED.
+            destruct (nc!fid0) eqn:NOT; inv NOT_COMPILED.
+            inv MATCHSTACK. inv MSF.
+            exists Zero. econstructor. split.
+            * left. apply plus_one. eapply Return_RTL; eauto; simpl.
+              ** unfold n_load, sbind. simpl. eauto.
+              ** unfold n_open_stackframe. simpl. eauto.
+              ** unfold n_save. simpl. eauto.
+              ** unfold n_check_compiled. simpl. rewrite NOT. eauto.
+            * eapply refl_match. auto.
+          + simpl in RETVAL. inv RETVAL.
+            simpl in OPEN_SF. unfold n_open_stackframe in OPEN_SF. simpl in OPEN_SF.
+            destruct top; inv OPEN_SF. destruct stk'; inv H0. destruct s; inv H1. destruct a, p, p0, p.
+            inv H0. simpl in SETRETVAL. unfold n_save in SETRETVAL. simpl in SETRETVAL. inv SETRETVAL.
+            simpl in NOT_COMPILED. unfold n_check_compiled in NOT_COMPILED. simpl in NOT_COMPILED.
+            destruct (nc!fid0) eqn:NOT; inv NOT_COMPILED.
+            inv MATCHSTACK. inv MSF.
+            exists Zero. econstructor. split.
+            * left. apply plus_one. eapply Return_RTL; eauto; simpl.
+              ** unfold n_load, sbind. simpl. eauto.
+              ** unfold n_open_stackframe. simpl. eauto.
+              ** unfold n_save. simpl. eauto.
+              ** unfold n_check_compiled. simpl. rewrite NOT. eauto.
+            * eapply refl_match. auto.
+        - destruct loc.
+          + simpl in RETVAL. repeat sdo_ok. unfold n_load in HDO. simpl in HDO. destruct top; inv HDO.
+            simpl in OPEN_SF. unfold n_open_stackframe in OPEN_SF. simpl in OPEN_SF.
+            destruct top; inv OPEN_SF. destruct stk'; inv H0. destruct s; inv H1. destruct a, p, p0, p.
+            inv H0. simpl in SETRETVAL. unfold n_save in SETRETVAL. simpl in SETRETVAL. inv SETRETVAL.
+            simpl in NOT_COMPILED. unfold n_check_compiled in NOT_COMPILED. simpl in NOT_COMPILED.
+            destruct (nc!fid0) eqn:NOT; inv NOT_COMPILED.
+            inv MATCHSTACK. inv MSF.
+            exists Zero. econstructor. split.
+            * left. apply plus_one. eapply Return_RTL_Block; eauto; simpl.
+              ** unfold n_load, sbind. simpl. eauto.
+              ** unfold n_open_stackframe. simpl. eauto.
+              ** unfold n_save. simpl. eauto.
+              ** unfold n_check_compiled. simpl. rewrite NOT. eauto.
+            * eapply refl_match. auto.
+          + simpl in RETVAL. inv RETVAL.
+            simpl in OPEN_SF. unfold n_open_stackframe in OPEN_SF. simpl in OPEN_SF.
+            destruct top; inv OPEN_SF. destruct stk'; inv H0. destruct s; inv H1. destruct a, p, p0, p.
+            inv H0. simpl in SETRETVAL. unfold n_save in SETRETVAL. simpl in SETRETVAL. inv SETRETVAL.
+            simpl in NOT_COMPILED. unfold n_check_compiled in NOT_COMPILED. simpl in NOT_COMPILED.
+            destruct (nc!fid0) eqn:NOT; inv NOT_COMPILED.
+            inv MATCHSTACK. inv MSF.
+            exists Zero. econstructor. split.
+            * left. apply plus_one. eapply Return_RTL_Block; eauto; simpl.
+              ** unfold n_load, sbind. simpl. eauto.
+              ** unfold n_open_stackframe. simpl. eauto.
+              ** unfold n_save. simpl. eauto.
+              ** unfold n_check_compiled. simpl. rewrite NOT. eauto.
+            * eapply refl_match. auto.
+         - destruct loc.
+          + simpl in RETVAL. repeat sdo_ok. unfold n_load in HDO. simpl in HDO. destruct top; inv HDO.
+            simpl in OPEN_SF. unfold n_open_stackframe in OPEN_SF. simpl in OPEN_SF.
+            destruct top; inv OPEN_SF. destruct stk'; inv H0.
+            2: { destruct s; inv H1. destruct a, p, p0, p. inv H0. }
+            inv MATCHSTACK.
+            exists Zero. econstructor. split.
+            * left. apply plus_one. eapply Return_EOE; eauto; simpl.
+              ** unfold n_load, sbind. simpl. eauto.
+              ** unfold n_open_stackframe. simpl. eauto.
+            * eapply refl_match; eauto. constructor.
+          + simpl in RETVAL. inv RETVAL.
+            simpl in OPEN_SF. unfold n_open_stackframe in OPEN_SF. simpl in OPEN_SF.
+            destruct top; inv OPEN_SF. destruct stk'; inv H0.
+            2: { destruct s; inv H1. destruct a, p, p0, p. inv H0. }
+            inv MATCHSTACK.
+            exists Zero. econstructor. split.
+            * left. apply plus_one. eapply Return_EOE; eauto; simpl.
+              ** unfold n_load, sbind. simpl. eauto.
+              ** unfold n_open_stackframe. simpl. eauto.
+            * eapply refl_match; eauto. constructor.
+        - destruct ms1, ms2. eapply addstk_same in TARGET as [s [APP SAME]]; eauto.
+          2: apply addstk_target.
+          eapply addstk_same in BUILD_RM as [s2 [APP2 SAME2]]; eauto.
+          2: apply addstk_build.
+          unfold find_function_ir in FINDOPTF.
+          unfold set_version, set_version_funlist in FINDF. simpl in FINDF.
+          rewrite FINDOPTF in FINDF.
+          poseq_destr ftgt fid.
+          + exists Zero. econstructor. split.
+            * left. apply plus_one. eapply Deopt; eauto; simpl.
+            * rewrite PTree.gss in FINDF. inv FINDF. rewrite base_version_set_version.
+              eapply refl_match; eauto. apply match_app. apply match_app. auto.
+          + exists Zero. econstructor. split.
+            * left. apply plus_one. eapply Deopt; eauto; simpl.
+              ** rewrite PTree.gso in FINDF; eauto.
+            * eapply refl_match; eauto. subst. apply match_app. apply match_app. auto.
+        - destruct ms1. eapply addstk_same in PRIM_CALL as [s [APP SAME]].
+          2: { unfold ASMinterpreter.prim_sem_dec. repeat addstk_auto. }
+          exists Zero. econstructor. split.
+          + left. apply plus_one. eapply RTL_prim; eauto.
+          + eapply refl_match. subst. apply match_app. auto.
+        - exists Zero. econstructor. split.
+          + left. apply plus_one. eapply RTL_end; eauto.
+          + eapply refl_match. auto.
+        - exists Zero. econstructor. split.
+          + left. apply plus_one. eapply RTL_block_end; eauto.
+          + eapply refl_match. auto.
+        - exists Zero. econstructor. split.
+          + left. apply plus_one. eapply Anchor_go_on; eauto.
+          + eapply refl_match. auto.
+        - exists Zero. econstructor. split.
+          + left. apply plus_one. eapply Anchor_deopt; eauto.
+          + eapply refl_match. auto.
+Admitted.
